Added a property of symmetric lenses, and refined the definitions of the block open and close operators.

utp/utp_blocks.thy
@@ -1,71 +1,89 @@
 section \<open> Blocks (Abstract Local Variables) \<close>
 
 theory utp_blocks
-  imports utp_rel_laws
+  imports utp_rel_laws utp_wp
 begin
 
 syntax
   "_slens_view" :: "logic \<Rightarrow> svid" ("\<V>[_]")
+  "_slens_coview" :: "logic \<Rightarrow> svid" ("\<C>[_]")
 
 translations
   "_slens_view a" => "\<V>\<^bsub>a\<^esub>"
+  "_slens_coview a" => "\<C>\<^bsub>a\<^esub>"
 
 subsection \<open> Extending and Contracting Substitutions \<close>
 
 definition subst_ext :: "(<'\<alpha>, '\<beta>> \<Longleftrightarrow> '\<gamma>) \<Rightarrow> ('\<alpha>, '\<gamma>) psubst" ("ext\<^sub>s") where
-"ext\<^sub>s a = (\<lambda> s. create\<^bsub>\<V>\<^bsub>a\<^esub>\<^esub> s)" \<comment> \<open> Extend state space by execution of create \<close>
-
-lemma subst_ext_alt_def [upred_defs]: "ext\<^sub>s a = \<lparr>\<^bold>v \<mapsto>\<^sub>s &\<^bold>v \<restriction>\<^sub>e \<V>\<^bsub>a\<^esub>\<rparr>"
-  unfolding subst_ext_def by (rel_auto)
+\<comment> \<open> Extend state space, setting local state to an arbitrary value \<close>
+[upred_defs]: "ext\<^sub>s a = \<lparr>&\<V>[a] \<mapsto>\<^sub>s &\<^bold>v, &\<C>[a] \<mapsto>\<^sub>s \<guillemotleft>undefined\<guillemotright>\<rparr>" 
 
 definition subst_con :: "(<'\<alpha>, '\<beta>> \<Longleftrightarrow> '\<gamma>) \<Rightarrow> ('\<gamma>, '\<alpha>) psubst" ("con\<^sub>s") where
-"con\<^sub>s a = (\<lambda> s. get\<^bsub>\<V>\<^bsub>a\<^esub>\<^esub> s)" \<comment> \<open> Contract the state space with get \<close>
+\<comment> \<open> Contract the state space with get \<close>
+"con\<^sub>s a = (\<lambda> s. get\<^bsub>\<V>\<^bsub>a\<^esub>\<^esub> s)"
 
-lemma subst_con_alt_def [upred_defs]: "con\<^sub>s a = \<lparr>\<^bold>v \<mapsto>\<^sub>s &\<^bold>v \<oplus>\<^sub>p \<V>\<^bsub>a\<^esub>\<rparr>"
+lemma subst_con_alt_def [upred_defs]: "con\<^sub>s a = \<lparr>\<^bold>v \<mapsto>\<^sub>s &\<V>[a]\<rparr>"
   unfolding subst_con_def by (rel_auto)
-
-lemma subst_res_ext_con: "\<sigma> \<restriction>\<^sub>s (\<V>\<^bsub>a\<^esub>) = con\<^sub>s a \<circ> \<sigma> \<circ> ext\<^sub>s a"
-  by (rel_simp)
 
 lemma subst_ext_con [usubst]: "psym_lens a \<Longrightarrow> con\<^sub>s a \<circ> ext\<^sub>s a = id"
   by (rel_simp)
 
-text \<open> Variables in the "global" state space will be retained after a state is contracted \<close>
+text \<open> Variables in the global state space will be retained after a state is contracted \<close>
 
 lemma subst_con_update_sublens [usubst]: 
   "\<lbrakk> psym_lens a; x \<subseteq>\<^sub>L \<V>\<^bsub>a\<^esub> \<rbrakk> \<Longrightarrow> con\<^sub>s a \<circ> subst_upd \<sigma> x v = subst_upd (con\<^sub>s a \<circ> \<sigma>) (x /\<^sub>L \<V>\<^bsub>a\<^esub>) v"
   by (simp add: subst_con_def usubst alpha, rel_simp)
 
-text \<open> Variables in the "local" state space will be lost after a state is contracted \<close>
+text \<open> Variables in the local state space will be lost after a state is contracted \<close>
 
 lemma subst_con_update_indep [usubst]: 
   "\<lbrakk> mwb_lens x; psym_lens a; \<V>\<^bsub>a\<^esub> \<bowtie> x \<rbrakk> \<Longrightarrow> con\<^sub>s a \<circ> subst_upd \<sigma> x v = (con\<^sub>s a \<circ> \<sigma>)"
   by (simp add: subst_con_alt_def usubst alpha)
 
 lemma subst_ext_apply [usubst]: "\<langle>ext\<^sub>s a\<rangle>\<^sub>s x = &x \<restriction>\<^sub>e \<V>\<^bsub>a\<^esub>"
-  by (rel_simp)
+  apply (rel_simp)
+  oops
 
 subsection \<open> Generic Blocks \<close>
 
-text \<open> We ensure that the initial values of local are arbitrarily chosen \<close>
+text \<open> We ensure that the initial values of local are arbitrarily chosen using the non-deterministic
+  choice operator. \<close>
 
 definition block_open :: "(<'a, 'c> \<Longleftrightarrow> 'b) \<Rightarrow> ('a, 'b) urel" ("open\<^bsub>_\<^esub>") where
-[upred_defs]: "block_open a = \<langle>ext\<^sub>s a\<rangle>\<^sub>a ;; ($\<V>[a]\<acute> =\<^sub>u $\<V>[a])"
+[upred_defs]: "block_open a = \<langle>ext\<^sub>s a\<rangle>\<^sub>a ;; \<C>[a] := *"
+
+lemma block_open_alt_def:
+  "sym_lens a \<Longrightarrow> block_open a = \<langle>ext\<^sub>s a\<rangle>\<^sub>a ;; ($\<V>[a]\<acute> =\<^sub>u $\<V>[a])"
+  by (rel_auto, metis lens_indep_vwb_iff sym_lens.put_region_coregion_cover sym_lens_def)
 
 definition block_close :: "(<'a, 'c> \<Longleftrightarrow> 'b) \<Rightarrow> ('b, 'a) urel" ("close\<^bsub>_\<^esub>") where
 [upred_defs]: "block_close a = \<langle>con\<^sub>s a\<rangle>\<^sub>a"
 
-lemma block_open_conv: 
-  "psym_lens a \<Longrightarrow> open\<^bsub>a\<^esub>\<^sup>- = close\<^bsub>a\<^esub>"
-  by (rel_auto)
+lemma wp_open_block [wp]: "psym_lens a \<Longrightarrow> open\<^bsub>a\<^esub> wp b = (\<^bold>\<exists> v \<bullet> \<lparr>&\<V>[a] \<mapsto>\<^sub>s &\<^bold>v, &\<C>[a] \<mapsto>\<^sub>s \<guillemotleft>v\<guillemotright>\<rparr> \<dagger> b)"
+  by (simp add: block_open_def subst_ext_def wp usubst unrest)
+
+lemma wp_close_block [wp]: "psym_lens a \<Longrightarrow> close\<^bsub>a\<^esub> wp b = con\<^sub>s a \<dagger> b"
+  by (simp add: block_close_def subst_ext_def wp usubst unrest)
+
+lemma block_open_conv:
+  "sym_lens a \<Longrightarrow> open\<^bsub>a\<^esub>\<^sup>- = close\<^bsub>a\<^esub>"
+  by (rel_auto, metis lens_indep_def sym_lens.put_region_coregion_cover sym_lens_def)
 
 lemma block_open_close:
   "psym_lens a \<Longrightarrow> open\<^bsub>a\<^esub> ;; close\<^bsub>a\<^esub> = II"
-  by (rel_auto, metis mwb_lens_def psym_lens.mwb_region weak_lens.create_get)
+  by (rel_auto)
+
+text \<open> I needed this property for the assignment open law below. \<close>
+
+lemma usubst_prop: "\<sigma> \<oplus>\<^sub>s a = [a \<mapsto>\<^sub>s uop \<sigma> &a]"
+  by (rel_simp)
 
 lemma block_assigns_open:
-  "sym_lens a \<Longrightarrow> \<langle>\<sigma>\<rangle>\<^sub>a ;; open\<^bsub>a\<^esub> = open\<^bsub>a\<^esub> ;; \<langle>\<sigma> \<oplus>\<^sub>s \<V>\<^bsub>a\<^esub>\<rangle>\<^sub>a"
-  by (rel_auto, metis mwb_lens_axioms_def mwb_lens_def sym_lens_def vwb_lens_def wb_lens_axioms_def wb_lens_def weak_lens.put_get)
+  "psym_lens a \<Longrightarrow> \<langle>\<sigma>\<rangle>\<^sub>a ;; open\<^bsub>a\<^esub> = open\<^bsub>a\<^esub> ;; \<langle>\<sigma> \<oplus>\<^sub>s \<V>\<^bsub>a\<^esub>\<rangle>\<^sub>a"
+  apply (wp_calc)
+  apply (simp add: usubst_prop usubst)
+  apply (rel_auto)
+  done
 
 lemma block_assign_local_close:
   "\<V>\<^bsub>a\<^esub> \<bowtie> x \<Longrightarrow> x := v ;; close\<^bsub>a\<^esub> = close\<^bsub>a\<^esub>"
